theories/CCMetaTheory.v
@@ -596,8 +596,16 @@ Proof.
       (* Maybe I should check what happens with the first rasimpl above
         as it might already be responsible for a divergence with asimpl.
         Divergence is also ok as long as it gets better.
+
+        TODO: [ρ >> var] should be unquoted as ⟨ ρ ⟩
+        This happens only with qsubst_comp (qsubst_ren ρ) s
+        which is exactly what you get from qsubst_compr_l so maybe that optim
+        was wrong?
+        Maybe I need to see substitutions as combinations of renamings,
+        then proper substs, then term → term things (just renamings again?).
        *)
       rasimpl.
+      fail.
       reflexivity.
   - rasimpl. constructor.
     + auto.
